lib/Sets.i.dfy
@@ -3,14 +3,14 @@ include "NativeTypes.s.dfy"
 module Sets {
   import opened NativeTypes 
 
-  lemma {:opaque} SetInclusionImpliesSmallerCardinality(a: set<uint64>, b: set<uint64>)
+  lemma {:opaque} SetInclusionImpliesSmallerCardinality<T>(a: set<T>, b: set<T>)
     requires a <= b
     ensures |a| <= |b|
   {
     assert b == a + (b - a);
   }
 
-  lemma {:opaque} SetInclusionAndEqualCardinalityImpliesSetEquality(a: set<uint64>, b: set<uint64>)
+  lemma {:opaque} SetInclusionAndEqualCardinalityImpliesSetEquality<T>(a: set<T>, b: set<T>)
     requires a <= b
     requires |a| == |b|
     ensures a == b
